{-# OPTIONS --without-K #-}
-- Two equivalent approached to define the advantage in
-- a (bit) guessing game
open import Data.Two
open import Data.Nat.NP hiding (_==_)
open import Data.Nat.Distance
open import Data.Product.NP

open import Function

open import Explore.Core
open import Explore.Properties
open import Explore.Summable
open import Explore.Sum
open import Explore.Product
open import Explore.Two

open import Relation.Binary.PropositionalEquality.NP

module Explore.GuessingGameFlipping
                 (R : Set)(sum : Sum R)(sum-ind : SumInd sum)(â… : ğŸš â†’ R â†’ ğŸš) where
  open Operators
  X Y : R â†’ ğŸš
  X = â… 0â‚‚
  Y = â… 1â‚‚
  R' = ğŸš Ã— R
  sum' : Sum R'
  sum' = ğŸšË¢ Ã—Ë¢ sum

  open FromSum    sum'    renaming (count to #'_)
  open FromSumInd sum-ind renaming (count to #_)

  G : R' â†’ ğŸš
  G (b , r) = b == â… b r

  1/2 : R' â†’ ğŸš
  1/2 = fst

  -- TODO use the library
  lemma : âˆ€ X â†’ sum (const 1) â‰¡ #(not âˆ˜ X) + # X
  lemma X = sum-ind P refl (Î» {a}{b} â†’ part1 {a}{b}) part2
    where
      count = FromSum.count

      P = Î» s â†’ s (const 1) â‰¡ count s (not âˆ˜ X) + count s X

      part1 : âˆ€ {sâ‚€ sâ‚} â†’ P sâ‚€ â†’ P sâ‚ â†’ P (Î» f â†’ sâ‚€ f + sâ‚ f)
      part1 {sâ‚€} {sâ‚} Psâ‚€ Psâ‚ rewrite Psâ‚€ | Psâ‚ = +-interchange (count sâ‚€ (not âˆ˜ X)) (count sâ‚€ X) (count sâ‚ (not âˆ˜ X)) (count sâ‚ X)

      part2 : âˆ€ x â†’ P (Î» f â†’ f x)
      part2 x with X x
      part2 x | 0â‚‚ = refl
      part2 x | 1â‚‚ = refl

  thm : dist (#' G) (#' 1/2) â‰¡ dist (# Y) (# X)
  thm = dist (#' G) (#' 1/2)
      â‰¡âŸ¨ cong (dist (#' G)) helper âŸ©
        dist (#' G) (#(not âˆ˜ X) + # X)
      â‰¡âŸ¨ refl âŸ© -- #' definition
        dist (# (_==_ 0â‚‚ âˆ˜ X) + # (_==_ 1â‚‚ âˆ˜ Y)) (# (not âˆ˜ X) + # X)
      â‰¡âŸ¨ refl âŸ© -- #' definition
        dist (# (not âˆ˜ X) + # Y) (# (not âˆ˜ X) + # X)
      â‰¡âŸ¨ dist-x+ (# (not âˆ˜ X)) (# Y) (# X) âŸ©
        dist (# Y) (# X)
      âˆ
    where
      open â‰¡-Reasoning

      helper = #' 1/2
             â‰¡âŸ¨ refl âŸ©
               sum (const 0) + sum (const 1)
             â‰¡âŸ¨ cong (Î» p â†’ p + sum (const 1)) sum-zero âŸ©
               sum (const 1)
             â‰¡âŸ¨ lemma X âŸ©
               # (not âˆ˜ X) + # X
             âˆ
