module Explore.Sum where

open import Type
open import Function.NP
import Relation.Binary.PropositionalEquality.NP as â‰¡
open â‰¡ using (_â‰¡_ ; _â‰—_ ; _â‰—â‚‚_)
open import Explore.Type
open import Explore.Product
open import Data.Product
open import Data.Nat.NP
open import Data.Nat.Properties
open import Data.Bool.NP renaming (Bool to ğŸš; true to 1b; false to 0b; toâ„• to ğŸšâ–¹â„•)
open Data.Bool.NP.Indexed

module FromSum {A : â˜…} (sum : Sum A) where
  Card : â„•
  Card = sum (const 1)

  count : Count A
  count f = sum (ğŸšâ–¹â„• âˆ˜ f)

module FromSumInd {A : â˜…}
                  {sum : Sum A}
                  (sum-ind : SumInd sum) where
  open FromSum sum public

  sum-ext : SumExt sum
  sum-ext = sum-ind (Î» s â†’ s _ â‰¡ s _) (â‰¡.congâ‚‚ _+_)

  sum-zero : SumZero sum
  sum-zero = sum-ind (Î» s â†’ s (const 0) â‰¡ 0) (â‰¡.congâ‚‚ _+_) (Î» _ â†’ â‰¡.refl)

  sum-hom : SumHom sum
  sum-hom f g = sum-ind (Î» s â†’ s (f +Â° g) â‰¡ s f + s g)
                        (Î» {sâ‚€} {sâ‚} pâ‚€ pâ‚ â†’ â‰¡.trans (â‰¡.congâ‚‚ _+_ pâ‚€ pâ‚) (+-interchange (sâ‚€ _) (sâ‚€ _) _ _))
                        (Î» _ â†’ â‰¡.refl)

  sum-mono : SumMono sum
  sum-mono = sum-ind (Î» s â†’ s _ â‰¤ s _) _+-mono_

  sum-lin : SumLin sum
  sum-lin f zero    = sum-zero
  sum-lin f (suc k) = â‰¡.trans (sum-hom f (Î» x â†’ k * f x)) (â‰¡.congâ‚‚ _+_ (â‰¡.refl {x = sum f}) (sum-lin f k))

  module _ (f g : A â†’ â„•) where
    open â‰¡.â‰¡-Reasoning

    sum-âŠ“-âˆ¸ : sum f â‰¡ sum (f âŠ“Â° g) + sum (f âˆ¸Â° g)
    sum-âŠ“-âˆ¸ = sum f                          â‰¡âŸ¨ sum-ext (f âŸ¨ aâ‰¡aâŠ“b+aâˆ¸b âŸ©Â° g) âŸ©
              sum ((f âŠ“Â° g) +Â° (f âˆ¸Â° g))     â‰¡âŸ¨ sum-hom (f âŠ“Â° g) (f âˆ¸Â° g) âŸ©
              sum (f âŠ“Â° g) + sum (f âˆ¸Â° g) âˆ

    sum-âŠ”-âŠ“ : sum f + sum g â‰¡ sum (f âŠ”Â° g) + sum (f âŠ“Â° g)
    sum-âŠ”-âŠ“ = sum f + sum g               â‰¡âŸ¨ â‰¡.sym (sum-hom f g) âŸ©
              sum (f +Â° g)                â‰¡âŸ¨ sum-ext (f âŸ¨ a+bâ‰¡aâŠ”b+aâŠ“b âŸ©Â° g) âŸ©
              sum (f âŠ”Â° g +Â° f âŠ“Â° g)      â‰¡âŸ¨ sum-hom (f âŠ”Â° g) (f âŠ“Â° g) âŸ©
              sum (f âŠ”Â° g) + sum (f âŠ“Â° g) âˆ

    sum-âŠ” : sum (f âŠ”Â° g) â‰¤ sum f + sum g
    sum-âŠ” = â„•â‰¤.trans (sum-mono (f âŸ¨ âŠ”â‰¤+ âŸ©Â° g)) (â„•â‰¤.reflexive (sum-hom f g))

  count-ext : CountExt count
  count-ext fâ‰—g = sum-ext (â‰¡.cong ğŸšâ–¹â„• âˆ˜ fâ‰—g)

  sum-const : âˆ€ k â†’ sum (const k) â‰¡ Card * k
  sum-const k
      rewrite â„•Â°.*-comm Card k
            | â‰¡.sym (sum-lin (const 1) k)
            | projâ‚‚ â„•Â°.*-identity k = â‰¡.refl

  module _ f g where
    count-âˆ§-not : count f â‰¡ count (f âˆ§Â° g) + count (f âˆ§Â° notÂ° g)
    count-âˆ§-not rewrite sum-âŠ“-âˆ¸ (ğŸšâ–¹â„• âˆ˜ f) (ğŸšâ–¹â„• âˆ˜ g)
                      | sum-ext (f âŸ¨ toâ„•-âŠ“ âŸ©Â° g)
                      | sum-ext (f âŸ¨ toâ„•-âˆ¸ âŸ©Â° g)
                      = â‰¡.refl

    count-âˆ¨-âˆ§ : count f + count g â‰¡ count (f âˆ¨Â° g) + count (f âˆ§Â° g)
    count-âˆ¨-âˆ§ rewrite sum-âŠ”-âŠ“ (ğŸšâ–¹â„• âˆ˜ f) (ğŸšâ–¹â„• âˆ˜ g)
                    | sum-ext (f âŸ¨ toâ„•-âŠ” âŸ©Â° g)
                    | sum-ext (f âŸ¨ toâ„•-âŠ“ âŸ©Â° g)
                    = â‰¡.refl

    count-âˆ¨â‰¤+ : count (f âˆ¨Â° g) â‰¤ count f + count g
    count-âˆ¨â‰¤+ = â„•â‰¤.trans (â„•â‰¤.reflexive (sum-ext (â‰¡.sym âˆ˜ (f âŸ¨ toâ„•-âŠ” âŸ©Â° g))))
                         (sum-âŠ” (ğŸšâ–¹â„• âˆ˜ f) (ğŸšâ–¹â„• âˆ˜ g))

module FromSumÃ—
         {A B}
         {sumá´¬     : Sum A}
         (sum-indá´¬ : SumInd sumá´¬)
         {sumá´®     : Sum B}
         (sum-indá´® : SumInd sumá´®) where

  module |A| = FromSumInd sum-indá´¬
  module |B| = FromSumInd sum-indá´®

  sumá´¬á´® = sumá´¬ Ã—-sum sumá´®

  sum-âˆ˜projâ‚â‰¡Card* : âˆ€ f â†’ sumá´¬á´® (f âˆ˜ projâ‚) â‰¡ |B|.Card * sumá´¬ f
  sum-âˆ˜projâ‚â‰¡Card* f
      rewrite |A|.sum-ext (|B|.sum-const âˆ˜ f)
            = |A|.sum-lin f |B|.Card

  sum-âˆ˜projâ‚‚â‰¡Card* : âˆ€ f â†’ sumá´¬á´® (f âˆ˜ projâ‚‚) â‰¡ |A|.Card * sumá´® f
  sum-âˆ˜projâ‚‚â‰¡Card* = |A|.sum-const âˆ˜ sumá´®

  sum-âˆ˜projâ‚ : âˆ€ {f} {g} â†’ sumá´¬ f â‰¡ sumá´¬ g â†’ sumá´¬á´® (f âˆ˜ projâ‚) â‰¡ sumá´¬á´® (g âˆ˜ projâ‚)
  sum-âˆ˜projâ‚ {f} {g} sumfâ‰¡sumg
      rewrite sum-âˆ˜projâ‚â‰¡Card* f
            | sum-âˆ˜projâ‚â‰¡Card* g
            | sumfâ‰¡sumg = â‰¡.refl

  sum-âˆ˜projâ‚‚ : âˆ€ {f} {g} â†’ sumá´® f â‰¡ sumá´® g â†’ sumá´¬á´® (f âˆ˜ projâ‚‚) â‰¡ sumá´¬á´® (g âˆ˜ projâ‚‚)
  sum-âˆ˜projâ‚‚ sumfâ‰¡sumg = |A|.sum-ext (const sumfâ‰¡sumg)

-- -}
-- -}
-- -}
-- -}
