module sum-properties where

open import Type
import Level as L
open L using (Lift)
open import Data.Empty using (⊥)
open import Data.Bool.NP
open Data.Bool.NP.Indexed
open import Data.Nat.NP
open import Data.Nat.Properties
open import Data.Product renaming (map to pmap)
open import Data.Sum
open import Relation.Binary.Product.Pointwise
open import Data.Maybe
open import Data.Unit using (⊤)
open import Function.NP
import Function.Inverse as Inv
open Inv using (_↔_)
open import Function.Related
open import Function.Related.TypeIsomorphisms.NP
open import Function.Equality using (_⟨$⟩_)

--open import sum
open import Search.Type
open import Search.Sum
open import Search.Derived using (sum-swap)
open import Search.Searchable renaming (Searchable to SumProp)
open import Search.Searchable.Fin
open import Search.Searchable.Product
open import Search.Searchable.Sum
open import Relation.Binary.Sum
import Relation.Binary.PropositionalEquality.NP as ≡
open ≡ using (_≡_ ; _≗_ ; _≗₂_)

module _M2 {A : ★} (μA : SumProp A) (f g : A → Bool) where

sum-ext₂ : ∀ {A B}{f g : A → B → ℕ}(μA : SumProp A)(μB : SumProp B) → f ≗₂ g → sum μA (sum μB ∘ f) ≡ sum μA (sum μB ∘ g)
sum-ext₂ μA μB f≗g = sum-ext μA (sum-ext μB ∘ f≗g)

CountStableUnderInjection : ∀ {A} → SumProp A → Set
CountStableUnderInjection μ = ∀ p → Injective p → CountStableUnder (count μ) p

#-StableUnderInjection : ∀ {A}{μ : SumProp A} → SumStableUnderInjection (sum μ) → CountStableUnderInjection μ
#-StableUnderInjection sui p p-inj f = sui p p-inj (toℕ ∘ f)

⊤SUI : SumStableUnderInjection (sum μ⊤)
⊤SUI f p x = ≡.refl

{-
stableMaybe : ∀ {A} (μA : SumProp A) → StableUnderInjection μA
                                     → StableUnderInjection (μMaybe μA)
stableMaybe {A} μA suiA f p p-inj with p nothing | ≡.inspect p nothing
... | nothing | ≡.[ eq ] = {!!}
  where h : ∀ x → p (just x) ≡ just {!!}
        h = {!!}
        p' : A → A
        p' x = {!p (just x)!}
        p'-inj : Injective p'
        p'-inj = {!!}
... | just pn | ≡.[ eq ] = ≡.trans (≡.cong (λ x → f nothing + x) (suiA (f ∘ just) p' p'-inj)) {!!}
  where p' : A → A
        p' x = maybe id pn (p (just x))
        p'-inj : Injective p'
        p'-inj = {!!}
        
SumsOk : ∀ {A B} → SumProp A → SumProp B → A ↔ B → ★
SumsOk μA μB iso = ∀ f → sum μA f ≡ sum μB (f ∘ from)
  where from = _⟨$⟩_ (Inv.Inverse.from iso)
        
module StableIso {A B}(μA : SumProp A)(μB : SumProp B)(iso : A ↔ B)
                 (sums-ok : SumsOk μA μB iso)
                 (suiB    : StableUnderInjection μB) where
  to : A → B
  to x = Inv.Inverse.to iso ⟨$⟩ x

  from : B → A
  from x = Inv.Inverse.from iso ⟨$⟩ x

  from-inj : Injective from
  from-inj = Inv.Inverse.injective (Inv.sym iso)

  to-inj : Injective to
  to-inj = Inv.Inverse.injective iso

  left-inv : from ∘ to ≗ id
  left-inv = Inv.Inverse.left-inverse-of iso

  stable : StableUnderInjection μA
  stable f p p-inj
    = sum μA f
    ≡⟨ sums-ok f ⟩
      sum μB (f ∘ from)
    ≡⟨ suiB (f ∘ from) (to ∘ p ∘ from) (from-inj ∘ p-inj ∘ to-inj) ⟩
      sum μB (f ∘ from ∘ to ∘ p ∘ from)
    ≡⟨ sum-ext μB (λ x → ≡.cong f (left-inv (p (from x)))) ⟩
      sum μB (f ∘ p ∘ from)
    ≡⟨ ≡.sym (sums-ok (f ∘ p)) ⟩
      sum μA (f ∘ p)
    ∎
    where open ≡.≡-Reasoning

record Iso1+ {A : Set}(μA : SumProp A) : ★₁ where
  constructor mk
  field
    B   : ★
    μB  : SumProp B
    iso : A ↔ Maybe B

  toMaybe : A → Maybe B
  toMaybe x = Inv.Inverse.to iso ⟨$⟩ x

  fromMaybe : Maybe B → A
  fromMaybe x = Inv.Inverse.from iso ⟨$⟩ x

  field
    sums-ok  : ∀ f → sum μA f ≡ sum (μMaybe μB) (f ∘ fromMaybe)

  from-inj : Injective fromMaybe
  from-inj = Inv.Inverse.injective (Inv.sym iso)

  to-inj : Injective toMaybe
  to-inj = Inv.Inverse.injective iso

  left-inv : fromMaybe ∘ toMaybe ≗ id
  left-inv = Inv.Inverse.left-inverse-of iso

  stable : StableUnderInjection (μMaybe μB) → StableUnderInjection μA
  stable suiMB = StableIso.stable μA (μMaybe μB) iso sums-ok suiMB

-- iso1+⊤ : Iso1+ μ⊤
-- iso1+⊤ = {!mk !}

iso1+Maybe : ∀ {A} (μA : SumProp A) → Iso1+ μA → Iso1+ (μMaybe μA)
iso1+Maybe {A} μA A≅1+ = mk A μA Inv.id (λ f → ≡.refl)

iso1+FinSuc : ∀ n → Iso1+ (μFinSuc (suc n))
iso1+FinSuc n = mk (Fin (suc n)) (μFinSuc n) Fin∘suc↔Maybe∘Fin (λ f → ≡.refl)
-}

infix 4 _≈_

record _≈_ {A B} (μA : SumProp A)(μB : SumProp B) : Set where
  constructor mk
  field
    iso : A ↔ B
  from : B → A
  from x = Inv.Inverse.from iso ⟨$⟩ x

  to : A → B
  to x = Inv.Inverse.to iso ⟨$⟩ x

  from-inj : Injective from
  from-inj = Inv.Inverse.injective (Inv.sym iso)

  to-inj : Injective to
  to-inj = Inv.Inverse.injective iso

  field
    sums-ok : ∀ f → sum μA f ≡ sum μB (f ∘ from)

  sums-ok' : ∀ f → sum μB f ≡ sum μA (f ∘ to)
  sums-ok' f = sum μB f
             ≡⟨ sum-ext μB (≡.cong f ∘ ≡.sym ∘ Inv.Inverse.right-inverse-of iso) ⟩
               sum μB (f ∘ to ∘ from)
             ≡⟨ ≡.sym (sums-ok (f ∘ to)) ⟩
               sum μA (f ∘ to)
             ∎
    where open ≡.≡-Reasoning

  StableUnder≈ : SumStableUnderInjection (sum μA) → SumStableUnderInjection (sum μB)
  StableUnder≈ μA-SUI p p-inj f
    = sum μB f
    ≡⟨ sums-ok' f ⟩
      sum μA (f ∘ to)
    ≡⟨ μA-SUI (from ∘ p ∘ to) (to-inj ∘ p-inj ∘ from-inj) (f ∘ to) ⟩
      sum μA (f ∘ to ∘ from ∘ p ∘ to)
    ≡⟨ ≡.sym (sums-ok' (f ∘ to ∘ from ∘ p)) ⟩
      sum μB (f ∘ to ∘ from ∘ p)
    ≡⟨ sum-ext μB (≡.cong f ∘ Inv.Inverse.right-inverse-of iso ∘ p) ⟩
      sum μB (f ∘ p)
    ∎
    where open ≡.≡-Reasoning

≈-refl : ∀ {A} (μA : SumProp A) → μA ≈ μA
≈-refl μA = mk Inv.id (λ f → ≡.refl)

≈-id : ∀ {A} {μA : SumProp A} → μA ≈ μA
≈-id = ≈-refl _

≈-sym : ∀ {A B}{μA : SumProp A}{μB : SumProp B} → μA ≈ μB → μB ≈ μA
≈-sym A≈B = mk (Inv.sym iso) sums-ok'
  where open _≈_ A≈B

≈-trans : ∀ {A B C}{μA : SumProp A}{μB : SumProp B}{μC : SumProp C} → μA ≈ μB → μB ≈ μC → μA ≈ μC
≈-trans A≈B B≈C = mk (iso B≈C Inv.∘ iso A≈B) (λ f → ≡.trans (sums-ok A≈B f) (sums-ok B≈C (f ∘ from A≈B)))
  where open _≈_

infix 2 _≈∎
infixr 2 _≈⟨_⟩_

_≈∎ : ∀ {A} (μA : SumProp A) → μA ≈ μA
_≈∎ = ≈-refl

_≈⟨_⟩_ : ∀ {A B C} (μA : SumProp A){μB : SumProp B}{μC : SumProp C} → μA ≈ μB → μB ≈ μC → μA ≈ μC
_ ≈⟨ A≈B ⟩ B≈C = ≈-trans A≈B B≈C

{-
Fin1≈⊤ : μFin 1 ≈ μ⊤
Fin1≈⊤ = mk iso sums-ok where
  open import Relation.Binary.Sum
  iso : _
  iso = (A⊎⊥↔A Inv.∘ Inv.id ⊎-cong Fin0↔⊥) Inv.∘ Fin∘suc↔⊤⊎Fin

  sums-ok : (_ : _) → _
  sums-ok f = ≡.refl
-}

⊤+Fin : ∀ {n pf} → μ⊤ ⊎-μ μFinSuc n ≈ μFinSuc (suc n)
⊤+Fin {zero} {()}
⊤+Fin {suc n} = mk iso sums-ok where
  iso : _
  iso = Inv.sym Fin∘suc↔⊤⊎Fin

  sums-ok : (_ : _) → _
  sums-ok f = ≡.refl

⊤×A≈A : ∀ {A}{μA : SumProp A} → μ⊤ ×-μ μA ≈ μA
⊤×A≈A = mk iso sums-ok where
  iso : _
  iso = ⊤×A↔A

  sums-ok : (_ : _) → _
  sums-ok f = ≡.refl

μFinSucPres : ∀ {m n} → m ≡ n → μFinSuc m ≈ μFinSuc n
μFinSucPres eq rewrite eq = ≈-refl _

μFinPres : ∀ {m n pfm pfn} → m ≡ n → μFinSuc m {pfm} ≈ μFinSuc n {pfn}
μFinPres eq rewrite eq = ≈-refl _

  {-
Maybe-Finable : ∀ {A} (μA : SumProp A) → Finable μA → Finable (μMaybe μA)
Maybe-Finable {A} μA finA = mk card iso sums-ok where
  module FinA = Finable finA
  card = suc FinA.FinCard

  |A| : ℕ
  |A| = suc (Finable.FinCard finA)

  iso : _
  iso = (⊤ ⊎ A)       ↔⟨ Inv.id ⊎-cong FinA.iso ⟩
        (⊤ ⊎ Fin |A|) ↔⟨ sym Fin∘suc↔⊤⊎Fin ⟩
        Fin (suc |A|) ∎
    where open EquationalReasoning

  sums-ok : (_ : _) → _
  sums-ok f = ≡.cong (λ x → f (inj₁ _) + x) (FinA.sums-ok _)
-}

_+μ-cong_ : ∀ {A B C D}{μA : SumProp A}{μB : SumProp B}{μC : SumProp C}{μD : SumProp D}
          → μA ≈ μC → μB ≈ μD → μA ⊎-μ μB ≈ μC ⊎-μ μD
A≈C +μ-cong B≈D = mk iso sums-ok where
  open import Relation.Binary.Sum
  iso : _
  iso = (_≈_.iso A≈C) ⊎-cong (_≈_.iso B≈D)

  sums-ok : (_ : _) → _
  sums-ok f = ≡.cong₂ _+_ (_≈_.sums-ok A≈C (f ∘ inj₁)) (_≈_.sums-ok B≈D (f ∘ inj₂))

+μ-assoc : ∀ {A B C}(μA : SumProp A)(μB : SumProp B)(μC : SumProp C)
         → (μA ⊎-μ μB) ⊎-μ μC ≈ μA ⊎-μ (μB ⊎-μ μC)
+μ-assoc μA μB μC = mk iso sums-ok where
  iso : _
  iso = ⊎-CMon.assoc _ _ _

  sums-ok : (_ : _) → _
  sums-ok f = ℕ°.+-assoc (sum μA (f ∘ inj₁ ∘ inj₁)) (sum μB (f ∘ inj₁ ∘ inj₂)) (sum μC (f ∘ inj₂))

+μ-comm : ∀ {A B}(μA : SumProp A)(μB : SumProp B)
        → μA ⊎-μ μB ≈ μB ⊎-μ μA
+μ-comm μA μB = mk iso sums-ok where
  iso : _
  iso = ⊎-CMon.comm _ _

  sums-ok : (_ : _) → _
  sums-ok f = ℕ°.+-comm (sum μA (f ∘ inj₁)) (sum μB (f ∘ inj₂))

_×μ-cong_ :  ∀ {A B C D}{μA : SumProp A}{μB : SumProp B}{μC : SumProp C}{μD : SumProp D}
          → μA ≈ μC → μB ≈ μD → μA ×-μ μB ≈ μC ×-μ μD
_×μ-cong_ {μA = μA}{μD = μD} A≈C B≈D = mk iso sums-ok where
  open import Relation.Binary.Product.Pointwise
  iso : _
  iso = _≈_.iso A≈C ×-cong _≈_.iso B≈D

  sums-ok : (_ : _) → _
  sums-ok f = ≡.trans (sum-ext μA (_≈_.sums-ok B≈D ∘ curry f))
                      (_≈_.sums-ok A≈C (λ a → sum μD (curry f a ∘ (_≈_.from B≈D))))

×μ-assoc : ∀ {A B C}(μA : SumProp A)(μB : SumProp B)(μC : SumProp C)
         → (μA ×-μ μB) ×-μ μC ≈ μA ×-μ (μB ×-μ μC)
×μ-assoc μA μB μC = mk iso sums-ok where
  iso : _
  iso = ×-CMon.assoc _ _ _

  sums-ok : (_ : _) → _
  sums-ok f = ≡.refl

×μ-comm : ∀ {A B}(μA : SumProp A)(μB : SumProp B)
        → μA ×-μ μB ≈ μB ×-μ μA
×μ-comm μA μB = mk iso sums-ok where
  iso : _
  iso = ×-CMon.comm _ _

  sums-ok : (_ : _) → _
  sums-ok f = sum-swap μA μB (curry f)

×+-distrib : ∀ {A B C}(μA : SumProp A)(μB : SumProp B)(μC : SumProp C)
           → (μA ⊎-μ μB) ×-μ μC ≈ (μA ×-μ μC) ⊎-μ (μB ×-μ μC)
×+-distrib μA μB μC = mk iso sums-ok where
  iso : _
  iso = ×⊎°.distribʳ _ _ _

  sums-ok : (_ : _) → _
  sums-ok f = ≡.refl

{-
_Suc-+_ : ∀ {m} → Suc m → ∀ n → Suc (m + n)
_Suc-+_ {zero}  () _
_Suc-+_ {suc m} _  _ = _

+-≈ : ∀ m n {pfm pfn} → (μFin m {pfm}) +μ (μFin n {pfn}) ≈ μFin (m + n) {pfm Suc-+ n}
+-≈ zero _ {()}
+-≈ _ zero {_} {()}
+-≈ (suc m) (suc n) = μFin (suc m) +μ μFin (suc n)
                    ≈⟨ {!!} ⟩
                      μFin (suc m + suc n)
                    ≈∎
-}

{-
+-≈ (suc zero) (suc n) = μFin 1 +μ μFin (suc n)
               ≈⟨ Fin1≈⊤ +μ-cong ≈-refl (μFin (suc n)) ⟩
                μ⊤ +μ μFinSuc n
              ≈⟨ ⊤+Fin ⟩
                μFinSuc (suc n)
              ≈∎
+-≈ (suc (suc m)) (suc n) = μFinSuc (suc m) +μ μFinSuc n
              ≈⟨ ≈-sym ⊤+Fin +μ-cong ≈-refl (μFinSuc n) ⟩
                (μ⊤ +μ μFinSuc m) +μ μFinSuc n
              ≈⟨ +μ-assoc μ⊤ (μFinSuc m) (μFinSuc n) ⟩
                μ⊤ +μ (μFinSuc m +μ μFinSuc n)
              ≈⟨ ≈-refl μ⊤ +μ-cong +-≈ (suc m) (suc n) ⟩
                μ⊤ +μ μFinSuc (m + suc n)
              ≈⟨ ⊤+Fin ⟩
                μFinSuc (suc m + suc n)
              ≈∎
              -}

{-
+-≈ : ∀ m n → (μFinSuc m) +μ (μFinSuc n) ≈ μFinSuc (m + suc n)
+-≈ zero n    = μFinSuc zero +μ μFinSuc n
              ≈⟨ Fin1≈⊤ +μ-cong ≈-refl (μFinSuc n) ⟩
                μ⊤ +μ μFinSuc n
              ≈⟨ ⊤+Fin ⟩
                μFinSuc (suc n)
              ≈∎
+-≈ (suc m) n = μFinSuc (suc m) +μ μFinSuc n
              ≈⟨ ≈-sym ⊤+Fin +μ-cong ≈-refl (μFinSuc n) ⟩
                (μ⊤ +μ μFinSuc m) +μ μFinSuc n
              ≈⟨ +μ-assoc μ⊤ (μFinSuc m) (μFinSuc n) ⟩
                μ⊤ +μ (μFinSuc m +μ μFinSuc n)
              ≈⟨ ≈-refl μ⊤ +μ-cong +-≈ m n ⟩
                μ⊤ +μ μFinSuc (m + suc n)
              ≈⟨ ⊤+Fin ⟩
                μFinSuc (suc m + suc n)
              ≈∎

×-≈ : ∀ m n → μFinSuc m ×μ μFinSuc n ≈ μFinSuc (n + m * suc n)
×-≈ zero n    = μFinSuc 0 ×μ μFinSuc n
              ≈⟨ Fin1≈⊤ ×μ-cong (≈-refl (μFinSuc n)) ⟩
                μ⊤ ×μ μFinSuc n
              ≈⟨ ⊤×A≈A ⟩
                μFinSuc n
              ≈⟨ μFinSucPres (ℕ°.+-comm 0 n) ⟩
                μFinSuc (n + 0)
              ≈∎
×-≈ (suc m) n = μFinSuc (suc m) ×μ μFinSuc n
              ≈⟨ ≈-sym ⊤+Fin ×μ-cong ≈-refl (μFinSuc n) ⟩
                (μ⊤ +μ μFinSuc m) ×μ μFinSuc n
              ≈⟨ ×+-distrib μ⊤ (μFinSuc m) (μFinSuc n) ⟩
                (μ⊤ ×μ μFinSuc n) +μ (μFinSuc m ×μ μFinSuc n)
              ≈⟨ ⊤×A≈A {μA = μFinSuc n} +μ-cong ×-≈ m n ⟩
                μFinSuc n +μ μFinSuc (n + m * suc n)
              ≈⟨ +-≈ n (n + m * suc n) ⟩
                μFinSuc (n + suc m * suc n)
              ≈∎

-- μA→B ≈ μFinSuc (m ^ n)
-- μB   ≈ μFinSuc m
-- μMaybe→ μA→B μB ≈ μFinSuc (m * m ^ n)

open import Data.Fin using (Fin ; zero ; suc)

Finable : ∀ {A} → SumProp A → Set
Finable μA = Σ ℕ λ FinCard → μA ≈ μFinSuc FinCard

⊤-Finable : Finable μ⊤
⊤-Finable = 0 , ≈-sym Fin1≈⊤

Fin-Finable : ∀ {n} → Finable (μFinSuc n)
Fin-Finable {n} = n , ≈-refl (μFinSuc n)

+-Finable : ∀ {A B}(μA : SumProp A)(μB : SumProp B) → Finable μA → Finable μB → Finable (μA +μ μB)
+-Finable μA μB (|A| , A≈) (|B| , B≈) = (|A| + suc |B|) ,
  ( μA +μ μB
  ≈⟨ A≈ +μ-cong B≈ ⟩
    μFinSuc |A| +μ μFinSuc |B|
  ≈⟨ +-≈ |A| |B| ⟩
    μFinSuc (|A| + suc |B|) ≈∎)

×-Finable : ∀ {A B}(μA : SumProp A)(μB : SumProp B) → Finable μA → Finable μB → Finable (μA ×μ μB)
×-Finable μA μB (|A| , A≈) (|B| , B≈) = (|B| + |A| * suc |B|) ,
  ( μA ×μ μB
  ≈⟨ A≈ ×μ-cong B≈ ⟩
    μFinSuc |A| ×μ μFinSuc |B|
  ≈⟨ ×-≈ |A| |B| ⟩
    μFinSuc (|B| + |A| * suc |B|)
  ≈∎)

module _M3 where
  open import bijection-fin
  open import Data.Fin using (Fin; zero; suc)
  open import Data.Vec.NP renaming (sum to vsum)

  sumFin : ∀ n → Sum (Fin n)
  sumFin n f = vsum (tabulate f)

  sumFin-spec : ∀ n → sumFin (suc n) ≗ sum (μFinSuc n)
  sumFin-spec zero    f = ℕ°.+-comm (f zero) 0
  sumFin-spec (suc n) f = ≡.cong (_+_ (f zero)) (sumFin-spec n (f ∘ suc))

  sumFinSUI : ∀ n f p → Injective p → sumFin n f ≡ sumFin n (f ∘ p)
  sumFinSUI n f p p-inj = count-perm f p (λ _ _ → p-inj)

  μFinSUI : ∀ {n} → StableUnderInjection (μFinSuc n)
  μFinSUI {n} p p-inj f rewrite ≡.sym (sumFin-spec n f)
                              | ≡.sym (sumFin-spec n (f ∘ p))
                              = sumFinSUI (suc n) f p p-inj
open _M3 public

StableIfFinable : ∀ {A} (μA : SumProp A) → Finable μA → StableUnderInjection μA
StableIfFinable μA (_ , A≈Fin)
  = _≈_.StableUnder≈ (≈-sym A≈Fin) μFinSUI

Decomposable : ★ → ★₁
Decomposable A = (A ↔ ⊤) ⊎ (∃ λ (B : ★) → A ↔ Maybe B)

open EquationalReasoning

dec-iso : ∀ {A B} → (A ↔ B) → Decomposable A → Decomposable B
dec-iso A↔B (inj₁ A↔⊤) = inj₁ (A↔⊤ Inv.∘ sym A↔B)
dec-iso A↔B (inj₂ (C , A↔MaybeC)) = inj₂ (C , A↔MaybeC Inv.∘ sym A↔B)

Maybe×⊎ : ∀ {A B : ★} → (Maybe A × B) ↔ (B ⊎ (A × B))
Maybe×⊎ {A} {B} = (Maybe A × B)   ↔⟨ Maybe↔⊤⊎ ×-cong Inv.id ⟩
                  ((⊤ ⊎ A) × B)   ↔⟨ ×⊎°.distribʳ B ⊤ A ⟩
                  (⊤ × B ⊎ A × B) ↔⟨ ⊤×A↔A ⊎-cong Inv.id ⟩
                  (B ⊎ (A × B))   ∎

dec× : ∀ {A B} → Decomposable A → Decomposable B → Decomposable (A × B)
dec× {A} {B} (inj₁ A↔⊤) dB = dec-iso (B      ↔⟨ sym ⊤×A↔A ⟩
                                     (⊤ × B) ↔⟨ sym A↔⊤ ×-cong Inv.id ⟩
                                     (A × B) ∎) dB
dec× {A} {B} dA (inj₁ B↔⊤) = dec-iso (A      ↔⟨ sym A×⊤↔A ⟩
                                     (A × ⊤) ↔⟨ Inv.id ×-cong sym B↔⊤ ⟩
                                     (A × B) ∎) dA
dec× {A} {B} (inj₂ (C , A↔1+C)) (inj₂ (D , B↔1+D))
  = inj₂ (_ , Maybe-⊎ Inv.∘ Maybe×⊎ Inv.∘ A↔1+C ×-cong B↔1+D)

dec+ : ∀ {A B} → Decomposable A → Decomposable B → Decomposable (A ⊎ B)
dec+ {A} {B} (inj₁ A↔⊤)         dB = inj₂ (B , sym Maybe↔⊤⊎ Inv.∘ A↔⊤ ⊎-cong Inv.id)
dec+ {A} {B} (inj₂ (C , A↔1+C)) dB = inj₂ ((C ⊎ B) , sym Maybe↔⊤⊎
                                               Inv.∘ ⊎-CMon.assoc ⊤ C B
                                               Inv.∘ (Maybe↔⊤⊎ Inv.∘ A↔1+C) ⊎-cong Inv.id)

{-
dB = dec-iso {!!} dB
  where dec : Decomposable (A × B)
{-
 -- B     + C×B
 -- 1×B   + C×B
 -- (1+C) × B
 -- A     × B
 -}

Stable× : ∀ {A} (μA : SumProp A) {B} (μB : SumProp B)
                (suiA : StableUnderInjection μA)
                (suiB : StableUnderInjection μB)
              → StableUnderInjection (μA ×μ μB)
Stable× μA μB suiA suiB = {!!}

        -- -}
        -- -}
        -- -}
        -- -}
